simplified the Hedge.Elem.denote function
It does not need LabelIn for the termination proof

Validator/Hedge/Elem.lean
@@ -110,74 +110,36 @@ theorem denote_elem_sizeOf_star_right {α: Type} {σ: Type} [SizeOf σ] {p: Rege
     simp only [List.cons.sizeOf_spec, gt_iff_lt]
     omega
 
--- denote_symbol_lift_take and denote_symbol_lift_drop is used by denote_elem to lift
---   a Φ predicate to work on an element of the original list:
--- * (denote_symbol: σ -> List.ElemOf xs -> Prop) -> (σ -> List.ElemOf (List.take n xs) -> Prop)
--- * (denote_symbol: σ -> List.ElemOf xs -> Prop) -> (σ -> List.ElemOf (List.drop n xs) -> Prop)
--- This works, because take and drop create infixes of a list and an element of an infix is a element.
--- We need these lifting functions to make the prove that denote_list = Regex.denote possible.
--- See denote_list_concat_n and denote_list_star_n for the exact detail.
-
-def denote_symbol_lift_take (n: Nat) (Φ: σ -> Hedge.LabelIn xs -> Prop): (σ -> Hedge.LabelIn (List.take n xs) -> Prop) :=
-  fun (s: σ) (y: Hedge.LabelIn (List.take n xs)) =>
-    Φ s (Hedge.LabelIn.mk y.val xs (by apply Hedge.labelin_take_is_labelelem))
-
-def denote_symbol_lift_drop (n: Nat) (Φ: σ -> Hedge.LabelIn xs -> Prop): (σ -> Hedge.LabelIn (List.drop n xs) -> Prop) :=
-  fun (s: σ) (y: Hedge.LabelIn (List.drop n xs)) =>
-    Φ s (Hedge.LabelIn.mk y.val xs (by apply Hedge.labelin_drop_is_labelelem))
-
-def lift_symbol {x: Hedge.Node α}
-  (Φ: φ -> LabelIn [x] -> Prop): (φ -> LabelIn x.getChildren -> Prop) :=
-  fun p hchildren => Φ p (by
-    clear Φ
-    clear p
-    clear φ
-    unfold LabelIn at *
-    cases hchildren with
-    | mk childlabel hchildren' =>
-    refine (Subtype.mk childlabel ?_)
-    cases x with
-    | mk label children =>
-    simp only [Node.getChildren] at *
-    unfold Hedge.LabelElem
-    simp only [List.flatMap]
-    simp only [List.map, List.flatten]
-    simp only [List.append_eq, List.append_nil]
-    simp only [Node.getLabels]
-    -- aesop?
-    simp_all only [List.mem_flatMap, List.mem_cons, or_true]
-  )
-
 -- Hedge.Elem.Rule.denote_elem is an alternative version of Hedge.Grammar.Rule.denote.
 -- The only other changes is that denote_elem contains unfolded versions of Language.or, Language.concat_n and Language.star_n.
 def Rule.denote_elem
   {α: Type} {φ: Type}
   (G: Hedge.Grammar n φ)
   (r: Hedge.Grammar.Rule n φ) (xs: Hedge α)
-  (Φ: φ -> Hedge.LabelIn xs -> Prop): Prop :=
+  (Φ: φ -> α -> Prop): Prop :=
   match r with
   | Regex.emptyset => Regex.Language.emptyset xs
   | Regex.emptystr => Regex.Language.emptystr xs
   | Regex.symbol (pred, ref) =>
     match xs with
     | [x] =>
-      (Φ pred (Hedge.LabelIn.self x))
-      /\ denote_elem G (G.lookup ref) x.getChildren (lift_symbol Φ)
+      (Φ pred x.getLabel)
+      /\ denote_elem G (G.lookup ref) x.getChildren Φ
     | _ => False
   | Regex.or r1 r2 =>
        (denote_elem G r1 xs Φ)
     \/ (denote_elem G r2 xs Φ)
   | Regex.concat r1 r2 =>
      ∃ (i: Fin (xs.length + 1)),
-       (denote_elem G r1 (List.take i xs) (denote_symbol_lift_take i Φ))
-    /\ (denote_elem G r2 (List.drop i xs) (denote_symbol_lift_drop i Φ))
+       (denote_elem G r1 (List.take i xs) Φ)
+    /\ (denote_elem G r2 (List.drop i xs) Φ)
   | Regex.star r1 =>
     match xs with
     | [] => True
     | (x'::xs') =>
        ∃ (i: Fin xs.length),
-         (denote_elem G r1 (List.take (i + 1) (x'::xs')) (denote_symbol_lift_take (i + 1) Φ))
-      /\ (denote_elem G (Regex.star r1) (List.drop (i + 1) (x'::xs')) (denote_symbol_lift_drop (i + 1) Φ))
+         (denote_elem G r1 (List.take (i + 1) (x'::xs')) Φ)
+      /\ (denote_elem G (Regex.star r1) (List.drop (i + 1) (x'::xs')) Φ)
   termination_by (xs, r)
   decreasing_by
     · apply decreasing_symbol
@@ -191,7 +153,7 @@ def Rule.denote_elem
 def Rule.denote {α: Type} {φ: Type}
   (G: Hedge.Grammar n φ) (Φ: φ -> α -> Prop)
   (r: Hedge.Grammar.Rule n φ) (xs: Hedge α): Prop :=
-  Rule.denote_elem G r xs (fun p x' => Φ p x'.val)
+  Rule.denote_elem G r xs (fun p x' => Φ p x')
 
 theorem denote_emptyset {α: Type} {φ: Type} (G: Hedge.Grammar n φ) (Φ: φ -> α -> Prop):
   Rule.denote G Φ Regex.emptyset = Regex.Language.emptyset := by
@@ -233,7 +195,7 @@ theorem denote_symbol {α: Type} {φ: Type} (G: Hedge.Grammar n φ) (Φ: φ -> �
   | nil =>
     rw [Rule.denote_elem]
     simp only [List.ne_cons_self, decide_eq_true_eq, false_and, exists_const, exists_false]
-    intro x Φ h
+    intro x h
     contradiction
   | cons x xs =>
     cases xs with
@@ -243,7 +205,7 @@ theorem denote_symbol {α: Type} {φ: Type} (G: Hedge.Grammar n φ) (Φ: φ -> �
       cases x with
       | mk label children =>
       simp only [Node.mk.injEq, ↓existsAndEq, and_true, exists_eq_left']
-      simp only [LabelIn.self, Node.getLabel]
+      simp only [Node.getLabel]
       simp_all only [eq_iff_iff, and_congr_right_iff]
       intro a
       obtain ⟨fst, snd⟩ := s
@@ -252,7 +214,7 @@ theorem denote_symbol {α: Type} {φ: Type} (G: Hedge.Grammar n φ) (Φ: φ -> �
     | cons x' xs =>
       rw [Rule.denote_elem]
       simp
-      intro x Φ h
+      intro x h
       simp at h
 
 theorem denote_or {α: Type} {φ: Type} (G: Hedge.Grammar n φ) (Φ: φ -> α -> Prop) (r1 r2: Rule n φ):
@@ -270,13 +232,13 @@ theorem denote_concat_n {α: Type} {φ: Type} (G: Hedge.Grammar n φ) (Φ: φ ->
   rfl
 
 theorem unfold_denote_elem_star_n {α: Type} {φ: Type} (G: Hedge.Grammar n φ) (Φ: φ -> α -> Prop) (r: Rule n φ) (xs: Hedge α):
-  Rule.denote_elem G (Regex.star r) xs (fun p x' => Φ p x'.val)
+  Rule.denote_elem G (Regex.star r) xs (fun p x' => Φ p x')
   = (match xs with
     | [] => True
     | (x'::xs') =>
        ∃ (n: Fin xs.length),
-         (Rule.denote_elem G r (List.take (n + 1) (x'::xs')) (denote_symbol_lift_take (n + 1) (fun p x' => Φ p x'.val)))
-      /\ (Rule.denote_elem G (Regex.star r) (List.drop (n + 1) (x'::xs')) (denote_symbol_lift_drop (n + 1) (fun p x' => Φ p x'.val)))) := by
+         (Rule.denote_elem G r (List.take (n + 1) (x'::xs')) Φ)
+      /\ (Rule.denote_elem G (Regex.star r) (List.drop (n + 1) (x'::xs')) Φ)) := by
   cases xs with
   | nil =>
     simp [Rule.denote_elem]
@@ -288,7 +250,7 @@ theorem unfold_denote_elem_star_n {α: Type} {φ: Type} (G: Hedge.Grammar n φ) 
       simp only [Rule.denote_elem]
 
 theorem denote_elem_star_n_iff {α: Type} {φ: Type} (G: Hedge.Grammar n φ) (Φ: φ -> α -> Prop) (r: Rule n φ) (xs: Hedge α):
-  Rule.denote_elem G (Regex.star r) xs (fun p x' => Φ p x'.val) <-> Regex.Language.star_n (fun xs' => Rule.denote_elem G r xs' (fun p x' => Φ p x'.val)) xs := by
+  Rule.denote_elem G (Regex.star r) xs (fun p x' => Φ p x') <-> Regex.Language.star_n (fun xs' => Rule.denote_elem G r xs' (fun p x' => Φ p x')) xs := by
   rw [<- eq_iff_iff]
   unfold Regex.Language.star_n
   rw [unfold_denote_elem_star_n]
@@ -300,11 +262,7 @@ theorem denote_elem_star_n_iff {α: Type} {φ: Type} (G: Hedge.Grammar n φ) (Φ
     congr
     ext n
     rw [<- eq_iff_iff]
-    unfold denote_symbol_lift_take
-    unfold denote_symbol_lift_drop
     congr
-    simp only
-    simp only [LabelIn.mk]
     simp only [List.length_cons, List.drop_succ_cons, eq_iff_iff]
     rw [<- denote_elem_star_n_iff]
   termination_by xs.length
